Shallow partially ported to the new style WPs to support allocation

examples/seplogic/Shallow.fst
@@ -4,42 +4,47 @@ open SepLogic.Heap
 
 module S = FStar.Squash
 
-unfold let memory = m:memory{defined m}
+let memory = m:memory{defined m}
 
 (* postcondition, a predicate on the return value and the output heap *)
-let post (a:Type) = a * memory -> Type0
+let post (a:Type) = a * heap -> Type0
 
 (* precondition, a predicate on the input heap *)
-let pre = memory -> Type0
+let pre = heap -> Type0
 
 (* wp *)
 let st_wp (a:Type) = post a -> pre
 
 (* result type parametrized by a post *)
-let result (a:Type) (post:post a) = x:(a * heap){post (fst x, heap_memory (snd x))}
+let result (h0:heap) (a:Type) (post:post a) = 
+  x_h:(a * heap){post x_h /\ fresh_or_old h0 (snd #a #heap x_h)}
 
 (* st computation, also parametrized by a post *)
 let st (a:Type) (wp:st_wp a) = 
-  post:post a -> h0:heap{wp post (heap_memory h0)} -> Tot (squash (result a post))
+  post:post a -> h0:heap{wp post h0} -> Tot (squash (result h0 a post))
 
 (* return *)
 let return (#a:Type) (x:a)
-  : st a (fun post m0 -> m0 == emp /\ post (x, m0))
+  : st a (fun post h0 -> heap_memory h0 == emp /\ post (x, h0))
   = fun post h0 -> S.return_squash (x, h0)
 
 (* frame wp by partitioning a heap whose memory is m into h0 and h1, and then prove post on the resulting heap and h1 *)
-let frame_wp0 (#a:Type) (wp:st_wp a) (post:memory -> (a * memory) -> Type0) (m m0 m1:memory) =
-  defined (m0 <*> m1) /\ m == (m0 <*> m1) /\ wp (post m1) m0
+let frame_wp0 (#a:Type) (wp:st_wp a) (post:heap -> (a * heap) -> Type0) (h:heap) (m0 m1:memory) =
+  defined (m0 <*> m1) /\ 
+  heap_memory h == (m0 <*> m1) /\ 
+  (let (h0,h1) = split_heap m0 m1 h in wp (post h1) h0)
 
-let frame_wp1 (#a:Type) (wp:st_wp a) (post:memory -> (a * memory) -> Type0) (m m0:memory) =
-  exists (m1:memory). frame_wp0 wp post m m0 m1
+let frame_wp1 (#a:Type) (wp:st_wp a) (post:heap -> (a * heap) -> Type0) (h:heap) (m0:memory) =
+  exists m1. frame_wp0 wp post h m0 m1
 
-let frame_wp (#a:Type) (wp:st_wp a) (post:memory -> (a * memory) -> Type0) (m:memory) =
-  exists (m0:memory). frame_wp1 wp post m m0
+let frame_wp (#a:Type) (wp:st_wp a) (post:heap -> (a * heap) -> Type0) (h:heap) =
+  exists m0. frame_wp1 wp post h m0
 
 (* the idea is to call frame_wp with (frame_post p)? yes, see frame below *)
-let frame_post (#a:Type) (p:post a) (m0:memory) ((x, m1):(a * memory)) = 
-  defined (m0 <*> m1) /\ p (x, m0 <*> m1)
+let frame_post (#a:Type) (p:post a) (h0:heap) : post a =
+  fun x_h1 -> 
+    let (x, h1) = x_h1 in 
+    defined (heap_memory h0 <*> heap_memory h1) /\ p (x, join h0 h1)
 
 let bind_exists
   (#a:Type)
@@ -50,63 +55,99 @@ let bind_exists
   : Tot (squash a)
   = S.bind_squash #(x:b & p x) #a h (fun (| x, p |) -> f x p)
 
-val frame: #a:Type -> #wp:st_wp a -> f:st a wp
+(*val frame: #a:Type -> #wp:st_wp a -> f:st a wp
          -> st a (fun post -> frame_wp wp (frame_post post))
-//Expanded out:
-//         st a (fun post m -> exists m0 m1. disjoint m0 m1 /\ m == m0 <*> m1 /\ wp (fun m0' -> disjoint m0' m1 /\ post (x, (join_tot h0' h1))) m0
 let frame #a #wp f = 
-  fun post h ->
-    assert (frame_wp wp (frame_post post) (heap_memory h));
-    let s = S.join_squash (S.get_proof (frame_wp wp (frame_post post) (heap_memory h))) in
-    bind_exists #(result a post) #memory #(frame_wp1 wp (frame_post post) (heap_memory h)) s (fun m0 s' -> 
-      assert (frame_wp1 wp (frame_post post) (heap_memory h) m0);
-      bind_exists #(result a post) #memory #(frame_wp0 wp (frame_post post) (heap_memory h) m0) s' (fun m1 _ -> 
-        assert (frame_wp0 wp (frame_post post) (heap_memory h) m0 m1);
-        let (h0,h1) = split_heap m0 m1 h in
-        let sqres : squash (result a (frame_post post (heap_memory h1))) = f (frame_post post (heap_memory h1)) h0 in 
-        S.bind_squash #(result a (frame_post post (heap_memory h1)))
-                      #(result a post)
+  fun post h -> 
+    assert (frame_wp wp (frame_post post) h); 
+    let s = S.join_squash (S.get_proof (frame_wp wp (frame_post post) h)) in 
+    bind_exists #(result h a post) #memory #(frame_wp1 wp (frame_post post) h) s (fun m0 s' -> 
+      assert (frame_wp1 wp (frame_post post) h m0); 
+      bind_exists #(result h a post) #memory #(frame_wp0 wp (frame_post post) h m0) s' (fun m1 _ -> 
+        assert (frame_wp0 wp (frame_post post) h m0 m1); 
+        let (h0,h1) = split_heap m0 m1 h in 
+        let sqres : squash (result h0 a (frame_post post h1)) = f (frame_post post h1) h0 in 
+        S.bind_squash #(result h0 a (frame_post post h1))
+                      #(result h a post)
                       sqres
-                      (fun (x_h0':result a (frame_post post (heap_memory h1))) -> 
+                      (fun (x_h0':result h0 a (frame_post post h1)) -> 
                          let (x, h0') = x_h0' in
                          let res = (x, join h1 h0') in 
-                         S.return_squash res)))
-      
+                         lemma_fresh_or_old_disjoint h0 h0' h1;
+                         lemma_fresh_or_old_sep h0 h0' h1;
+                         S.return_squash res)))*)
+(*
+#set-options "--z3rlimit_factor 1 --max_fuel 0 --max_ifuel 0"
+
 val bind (#a:Type) (#wp1:st_wp a)
          (#b:Type) (#wp2:a -> st_wp b)
          (f:st a wp1)
          (g: (x:a -> st b (wp2 x)))
-    : st b (fun post m ->
-            frame_wp wp1 (frame_post (fun (x, m1) ->
-              frame_wp (wp2 x) (frame_post post) m1)) m)
+    : st b (fun post h ->
+            frame_wp wp1 (frame_post (fun (x, h1) ->
+              frame_wp (wp2 x) (frame_post post) h1)) h)
+              
+(*
+bind f g post :
+-> h0:heap{frame_wp wp1 (frame_post (fun (x, h1) -> frame_wp (wp2 x) (frame_post post) h1)) h0} 
+-> Tot (squash (result h0 a post))
+*)
+
+(*
+frame f (fun (x, h1) -> frame_wp (wp2 x) (frame_post post) h1) :
+-> h0:heap{frame_wp wp1 (frame_post (fun (x, h1) -> frame_wp (wp2 x) (frame_post post) h1)) h0} 
+-> Tot (squash (x_h:(a * heap){(fun (x, h1) -> frame_wp (wp2 x) (frame_post post) h1) x_h /\ fresh_or_old h0 (snd x_h)}))
+*)
+
+(*
+frame (g x) post :
+-> h1:heap{frame_wp (wp2 x) (frame_post post) h1}
+-> Tot (squash (x_h':(a * heap){post x_h' /\ fresh_or_old h1 (snd x_h')}))
+*)
+
 let bind #a #wp1 #b #wp2 f g =
-    fun post h ->
-      let sq_1 : squash (result a (fun (x, m1) -> frame_wp (wp2 x) (frame_post post) m1)) =
-        frame f (fun (x, m1) -> frame_wp (wp2 x) (frame_post post) m1) h in
-      S.bind_squash sq_1 (fun (x, m1) ->
-      frame (g x) post m1)
+    fun post h0 ->
+      assert (frame_wp wp1 (frame_post (fun (x, h1) -> frame_wp (wp2 x) (frame_post post) h1)) h0);
+      let sq_1 : squash (result h0 a (fun (x, h1) -> frame_wp (wp2 x) (frame_post post) h1)) =
+        frame f (fun (x, h1) -> frame_wp (wp2 x) (frame_post post) h1) h0 in 
+      S.bind_squash #(result h0 a (fun (x, h1) -> frame_wp (wp2 x) (frame_post post) h1)) #(result h0 b post) sq_1 (fun (x, h1) -> 
+        assert (frame_wp (wp2 x) (frame_post post) h1);
+        assert (fresh_or_old h0 h1);
+        let sq_2 : squash (result h1 b post) = 
+          frame (g x) post h1 in 
+        S.bind_squash #(result h1 b post) #(result h0 b post) sq_2 (fun (y_h:result h1 b post) ->
+          let (y, h2) : x_h:(b * heap){post x_h /\ fresh_or_old h0 (snd #b #heap x_h)} = y_h in
+          assert (post (y, h2));
+          assert (fresh_or_old h1 h2);
+          lemma_fresh_or_old_trans h0 h1 h2; 
+          assert (fresh_or_old h0 h2);
+          let res : squash (result h0 b post) = (y, h2) post in 
+          res))*)
 
 let alloc (#a:Type0) (x:a)
-  : st (ref a) (fun post m0 -> m0 == emp /\ (forall r m1 . m1 == (r |> x) ==> post (r, m1)))
+  : st (ref a) (fun post h0 -> heap_memory h0 == emp /\ (let (r,h1) = alloc h0 x in post (r, h1)))
   = fun post h0 ->
       let (r,h1) = alloc h0 x in
+      lemma_fresh_or_old_alloc x h0;
       S.return_squash (r,h1)
 
 let dealloc (#a:Type0) (r:ref a)
-  : st unit (fun post m0 -> (exists x . m0 == (r |> x)) /\ post ((), emp))
+  : st unit (fun post h0 -> (exists x . heap_memory h0 == (r |> x)) /\ hcontains h0 r /\ post ((), dealloc h0 r))
   = fun post h0 -> 
         assert (mcontains (heap_memory h0) r);
         let h1 = dealloc h0 r in
+        lemma_fresh_or_old_dealloc r h0;
         S.return_squash ((), h1)
 
 let read (#a:Type0) (r:ref a)
-  : st a (fun post m0 -> (exists (x:a). m0 == (r |> x) /\ post (x, m0)))
+  : st a (fun post h0 -> (exists (x:a). heap_memory h0 == (r |> x) /\ post (x, h0)))
   = fun post h0 -> 
       assert (mcontains (heap_memory h0) r);
       S.return_squash (sel h0 r, h0)
 
 let write (#a:Type0) (r:ref a) (v:a)
-  : st unit (fun post m0 -> (exists (x:a). m0 == (r |> x) /\ post ((), (r |> v))))
+  : st unit (fun post h0 -> (exists (x:a). heap_memory h0 == (r |> x) /\ hcontains h0 r /\ post ((), upd h0 r v)))
     = fun post h0 -> 
         assert (mcontains (heap_memory h0) r);
+        lemma_fresh_or_old_upd r v h0;
         S.return_squash ((), upd h0 r v)
